Have added signed and unsigned orderings:
Name                       Function  Symbol
-------------------------------------------
Less                       word_lt   <
Less or equal              word_le   <=
Greater                    word_gt   >
Greater or equal           word_ge   >=
Unsigned less              word_lo   <.
Unsigned less or equal     word_ls   <=.
Unsigned Greater           word_hi   >.
Unsigned Greater or equal  word_hs   >=.

They are defined in terms of the NZCV
(Negative, Zero, Carry and Overflow) flags
(after subtraction) but are related to
the natural number orderings.

Two extra constants are also added.
Lowest 2's complement value:  word_L (= n2w (2 EXP HB))
Highest 2's complement value: word_H (= n2w (2 EXP HB - 1))
where HB is the MSB bit position.

word_T_def and word_T have been changed, so as to be
more useful in proofs.

A few basic theorems about these orderings
have been added.  More may follow?  The compset
in wordFunctorLib has been updated.

src/n_bit/wordFunctorLib.sml
@@ -3,6 +3,8 @@ functor wordFunctorLib (structure wordTheory : sig
   val WL_def : Thm.thm
   val word_0 : Thm.thm
   val word_1 : Thm.thm
+  val word_L_def : Thm.thm
+  val word_H_def : Thm.thm
   val word_T : Thm.thm
   val MOD_WL_EVAL : Thm.thm
   val MSBn_def : Thm.thm
@@ -26,6 +28,14 @@ functor wordFunctorLib (structure wordTheory : sig
   val w2n_EVAL : Thm.thm
   val MSB_EVAL2 : Thm.thm
   val LSB_EVAL2 : Thm.thm
+  val LT_EVAL : Thm.thm
+  val LE_EVAL : Thm.thm
+  val GT_EVAL : Thm.thm
+  val GE_EVAL : Thm.thm
+  val LO_EVAL : Thm.thm
+  val LS_EVAL : Thm.thm
+  val HI_EVAL : Thm.thm
+  val HS_EVAL : Thm.thm
 end) : sig
   include Abbrev
 
@@ -53,7 +63,9 @@ val sn = Arbnum.toString wl;
 val word_compset =
   let val rws = reduceLib.num_compset()
       val _ = add_thms
-     [THE_WL, HB_def, word_0, word_1, word_T,
+     [LT_EVAL, LE_EVAL, GT_EVAL, GE_EVAL,
+      LO_EVAL, LS_EVAL, HI_EVAL, HS_EVAL,
+      THE_WL, HB_def, word_0, word_1, word_L_def, word_H_def, word_T,
       MOD_WL_EVAL, w2n_EVAL,
       ADD_EVAL2, MUL_EVAL2, word_sub,
       REDUCE_RULE ONE_COMP_EVAL2,
